TabularTypeInterpreter/F⊗⊕ω/Lemmas.lean
@@ -1,2 +1,3 @@
+import TabularTypeInterpreter.«F⊗⊕ω».Lemmas.Kind
 import TabularTypeInterpreter.«F⊗⊕ω».Lemmas.Type
 import TabularTypeInterpreter.«F⊗⊕ω».Lemmas.Value
